\documentclass{article}
\usepackage{amsmath}

\begin{document}

% Image 1 content
Let $G$ be a group. Let $H \lhd G$. Let $K \leq G$ such that $K/H = G/H$.

We have:
\begin{align*}
|G| &= |H| \cdot |K/H| \\
&= |H| \cdot |G/H| \\
&= |H| \cdot \frac{|G|}{|H|} \\
&= |G|
\end{align*}

Now consider:
\begin{align*}
N_G(K) &= \{ g \in G \mid gKg^{-1} = K \} \\
N_H(K) &= \{ h \in H \mid hKh^{-1} = K \}
\end{align*}

Since $K \leq G$ and $H \lhd G$, we have $K \cap H \lhd K$.

Also, since $K/H = G/H$, we have $KH = G$.

Now, if $k \in K$ and $h \in H$, then:
\[
khk^{-1} \in H \quad \text{(since $H \lhd G$)}
\]
and
\[
khk^{-1} \in K \quad \text{(since $K \leq G$ and $h \in H \leq G$)}
\]
Therefore $khk^{-1} \in K \cap H$.

So $K$ normalizes $H$, and $H$ normalizes $K$.

Thus $N_G(K) \geq H$ and $N_H(K) = H \cap N_G(K)$.

Since $K/H = G/H$, we have $|G/K| = |H/(K \cap H)|$.

Therefore:
\[
|N_G(K)| = |H| \cdot |N_G(K)/H|
\]

\end{document}