\documentclass{article}
\usepackage{amsmath}
\usepackage{amssymb}

\begin{document}

Let $G$ be a group and $H \triangleleft G$. Let $K \leq G$ such that $H \subseteq K$. Then:

\begin{enumerate}
    \item $K/H \triangleleft G/H$ if and only if $K \triangleleft G$
    \item $(G/H)/(K/H) \cong G/K$
\end{enumerate}

Proof of (1):

($\Rightarrow$) Assume $K/H \triangleleft G/H$. Then for all $gH \in G/H$, we have:
\[
(gH)(K/H)(gH)^{-1} = K/H
\]
This implies $gKg^{-1} \subseteq K$, so $K \triangleleft G$.

($\Leftarrow$) Assume $K \triangleleft G$. Then for all $g \in G$, we have $gKg^{-1} = K$. Therefore:
\[
(gH)(K/H)(gH)^{-1} = (gKg^{-1})/H = K/H
\]
So $K/H \triangleleft G/H$.

Proof of (2):

Define $\phi: G/H \to G/K$ by $\phi(gH) = gK$. This is well-defined since if $gH = g'H$, then $g^{-1}g' \in H \subseteq K$, so $gK = g'K$.

$\phi$ is a homomorphism:
\[
\phi(gH \cdot g'H) = \phi(gg'H) = gg'K = (gK)(g'K) = \phi(gH)\phi(g'H)
\]

$\phi$ is surjective: For any $gK \in G/K$, we have $\phi(gH) = gK$.

The kernel of $\phi$ is:
\[
\ker\phi = \{gH \in G/H : \phi(gH) = K\} = \{gH : gK = K\} = \{gH : g \in K\} = K/H
\]

By the First Isomorphism Theorem:
\[
(G/H)/\ker\phi \cong \operatorname{im}\phi
\]
So:
\[
(G/H)/(K/H) \cong G/K
\]

\end{document}